src3.0/Vellvm/Dominators/dom_type.v
@@ -7,10 +7,6 @@ Module DomDS := Dataflow_Solver_Var_Top(AtomNodeSet).
 
 Section A.
 
-Variable bound : ListSet.set atom.
-
-Definition answer := Maps.AMap.t (DomDS.dt bound).
-
 End A.
 
 End Dom_Kildall.
