src3.0/Vellvm/opsem_wf.v
@@ -547,17 +547,13 @@ Proof.
   unfold inscope_of_tmn in Hinscope.
   unfold inscope_of_tmn. unfold inscope_of_cmd, inscope_of_id.
   destruct F as [[f t i0 la va] bs].
-  remember (dom_analyze (fdef_intro (fheader_intro f t i0 la va) bs)) as Doms.
-  remember (Doms !! l3)as defs3.
-  remember (Doms !! l')as defs'.
-  destruct defs3 as [contents3 inbound3].
-  destruct defs' as [contents' inbound'].
 
-  assert (incl contents' (l3::contents3)) as Hsub.
-    clear - HBinF Hsucc Heqdefs3 Heqdefs' HeqDoms Huniq HwfF.
+  assert (incl (dom_query (fdef_intro (fheader_intro f t i0 la va) bs) l')
+     (l3::(dom_query (fdef_intro (fheader_intro f t i0 la va) bs) l3))) as Hsub.
+    clear - HBinF Hsucc Huniq HwfF.
     eapply dom_successors; eauto.
 
-  assert (J1:=inbound').
+  assert (J1:=dom_query_in_bound (fheader_intro f t i0 la va) bs l').
   apply fold_left__bound_blocks with (init:=getPhiNodesIDs ps' ++
     getArgsIDs la)(fh:=fheader_intro f t i0 la va)(bs:=bs) (l0:=l') in J1.
   destruct J1 as [r J1].
@@ -1870,25 +1866,26 @@ Proof.
     split.
       destruct f as [[]]. eapply initLocals__wf_lc; eauto.
     split.
+    Case "1".
      assert (ps'=nil) as EQ.
        eapply entryBlock_has_no_phinodes with (s:=S); eauto.
      subst.
      apply dom_entrypoint in H2.
      destruct cs'.
-       unfold inscope_of_tmn.
-       remember ((dom_analyze f) !! l') as R.
-       destruct R. simpl in H2. subst.
+     SCase "1.1".
+       unfold inscope_of_tmn. rewrite H2. simpl.
        destruct f as [[]].
        eapply preservation_dbCall_case; eauto using wf_params_spec.
 
+     SCase "1.2".
        unfold inscope_of_cmd, inscope_of_id.
        rewrite init_scope_spec1; auto.
-       remember ((dom_analyze f) !! l') as R.
-       destruct R. simpl. simpl in H2. subst.
+       rewrite H2. simpl.
        destruct (eq_atom_dec (getCmdLoc c) (getCmdLoc c)) as [|n];
          try solve [contradict n; auto].
        destruct f as [[]].
        eapply preservation_dbCall_case; eauto using wf_params_spec.
+    Case "2".
     exists l'. exists ps'. exists nil. simpl_env. auto.
 Qed.
 
